fixed all existing admits

fairness/lawyer/obligations_model.v
@@ -1,6 +1,5 @@
-From trillium.fairness Require Import fairness.
-From iris.algebra Require Import auth gmap gset excl gmultiset big_op mono_nat.
 From stdpp Require Import namespaces. 
+From trillium.fairness Require Import fairness locales_helpers.
 From trillium.fairness.lawyer Require Import obls_utils.
 
 
@@ -20,13 +19,14 @@ Class ObligationsParams
   opar_l0: Level;
   opar_l0_least: forall l, l ≠ opar_l0 -> opar_lvl_lt opar_l0 l;
   
-  opar_loc_eqdec :> EqDecision Locale;
-  opar_loc_cnt :> Countable Locale;
 }. 
 
 
 Section Model.
   Context `(OP: ObligationsParams Degree Level Locale LIM_STEPS).
+  (* opar_loc_eqdec :> EqDecision Locale; *)
+  (* opar_loc_cnt :> Countable Locale; *)
+  Context `{Countable Locale}. 
 
   Definition Phase := namespace. 
   Definition phase_le : Phase -> Phase -> Prop :=
@@ -185,104 +185,7 @@ Section Model.
   Definition ObligationsModel: Model :=
     {| mtrans := om_trans |}. 
 
-End Model.
 
-
-Section ObligationsRepr.
-  Context {DegO LevelO: ofe}.
-  Context `{OfeDiscrete DegO} `{OfeDiscrete LevelO} `{@LeibnizEquiv (ofe_car LevelO) (ofe_equiv LevelO)}.
-
-  Let Degree := ofe_car DegO.
-  Let Level := ofe_car LevelO.
-
-  (* Context {Locale: Type}. *)
-  Context {Λ: language}.
-  (* Context `{Countable (locale Λ)}.  *)
-  Let Locale := locale Λ. 
-  Context {LIM_STEPS: nat}.
-  Context (OP: ObligationsParams Degree Level Locale LIM_STEPS).
-  Let OM := ObligationsModel OP.
-
-  Let phO := listO positiveO. 
-  Let cpO := prodO phO DegO. 
-  Let sstR := prodR (agreeR LevelO) (excl' boolO).
- 
-  Let epO := prodO (prodO natO phO) DegO.
-
-  (* From iris.algebra.lib Require Import gset_bij.  *)
-  From iris.algebra.lib Require Import gset_bij.
-  From iris.base_logic.lib Require Import gset_bij.
-
-  Class ObligationsPreGS Σ := {
-      obls_pre_cps :> inG Σ (authUR (gmultisetUR cpO));
-      obls_pre_sigs :> inG Σ (authUR (gmapUR SignalId sstR));
-      obls_pre_obls :> inG Σ (authUR (gmapUR Locale (exclR (gsetUR natO))));
-      obls_pre_eps :> inG Σ (authUR (gsetUR epO)); (* allowing duplication of eps *)
-      obls_pre_phs :> inG Σ (authUR (gmapUR Locale (exclR phO)));
-      obls_pre_lb :> inG Σ mono_natUR;
-      si_obls_in :> gset_bijG Σ (locale Λ) Phase;
-  }.
-  Class ObligationsGS Σ := {
-      obls_pre :> ObligationsPreGS Σ;
-      obls_cps: gname;
-      obls_sigs: gname;
-      obls_obls: gname;
-      obls_eps: gname;
-      obls_phs: gname;
-      obls_exc_lb: gname;
-      (* obls_bij: gname; *)
-  }.  
-
-  Definition sig_map_repr smap: gmapUR SignalId sstR :=
-    (fun '(l, b) => (to_agree l, Excl' b)) <$> smap. 
-    (* [^op map] sg ↦ sst ∈ smap, {[ sg := (to_agree sst.1, Excl' sst.2) ]}. *)
-
-  Definition obls_map_repr (omap: gmap Locale (gset SignalId)):
-    gmapUR Locale (exclR (gsetUR natO)) :=
-    Excl <$> omap.
-
-  Definition phases_repr (pmap: gmap Locale Phase):
-    gmapUR Locale (exclR phO) :=
-    fmap Excl pmap (FMap := gmap_fmap).
-  
-  (* Context `{ObligationsGS Σ}.  *)
-  (* Set Printing All. *)
-
-  Definition eps_repr (eps: gset ExpectPermission): gsetUR epO :=
-    eps.
-
-  Definition cps_repr (cps: gmultiset (@CallPermission Degree)): (gmultisetUR cpO) := cps.
-
-  (* Definition obls_repr (obls: gmap Locale (gset SignalId)):  *)
-  
-  (* Definition obls_msi `{ObligationsGS Σ} (ps: ProgressState OP): iProp Σ := *)
-  (*   own obls_eps ((● (eps_repr $ ps_eps OP ps)): authUR (gsetUR epO)) *)
-  (* .  *)
-  Definition obls_msi `{ObligationsGS Σ} (ps: ProgressState OP): iProp Σ :=
-    own obls_cps (● (cps_repr $ ps_cps OP ps)) ∗
-    own obls_sigs (● (sig_map_repr $ ps_sigs OP ps)) ∗
-    own obls_obls (● (obls_map_repr $ ps_obls OP ps)) ∗
-    own obls_eps (● (eps_repr $ ps_eps OP ps)) ∗
-    own obls_phs (● (phases_repr $ ps_phases OP ps)) ∗
-    own obls_exc_lb (●MN (ps_exc_bound OP ps))
-  . 
-  
-  From trillium.fairness Require Import execution_model.
-  From iris.proofmode Require Import tactics.
-
-  Definition locales_of_cfg (c: cfg Λ): gset (locale Λ) :=
-        list_to_set (locales_of_list c.1).
-
-  Definition threads_own_obls (c: cfg Λ) (δ: mstate OM) (* m *) :=
-    (* bij (locales_of_cfg c) (dom $ ps_obls OP δ).  *)
-    
-    (* forall ζ, ζ ∈ dom (ps_obls OP δ) <-> is_Some (from_locale c.1 ζ). *)
-    
-    (* gset_bijective m /\  *)
-    (* set_map fst m = (locales_of_cfg c) /\ *)
-    (* set_map snd m = (dom $ ps_obls OP δ).  *)
-    locales_of_cfg c = dom $ ps_obls OP δ. 
-    
     
   (* Lemma burns_cp_th_obls_pres c τ δ1 δ2 d *)
   (*   (BURN: burns_cp OP δ1 τ δ2 d) *)
@@ -335,10 +238,10 @@ Section ObligationsRepr.
   (*   then dom (ps_obls OP δ) = (R ∖ {[ fork_left θ; fork_right θ ]} ∪ {[ θ ]}) /\ {[ fork_left θ; fork_right θ ]} ⊆ R *)
   (*   else dom (ps_obls OP δ) = R.  *)
 
-  Definition obls_eq δ1 R := dom $ ps_obls OP δ1 = R.
+  Definition obls_eq δ1 R := dom $ ps_obls δ1 = R.
       
   Lemma loc_step_obls_pres δ1 δ2 R θ
-    (LSTEP: loc_step OP δ1 θ δ2)
+    (LSTEP: loc_step δ1 θ δ2)
     (OBLS_CORR: obls_eq δ1 R)
     (* (DOMτ: is_Some (from_locale c.1 τ)): *)
     :
@@ -346,7 +249,7 @@ Section ObligationsRepr.
   Proof using.
     (* clear H H0 H1.  *)
     clear -LSTEP OBLS_CORR. 
-    add_case (dom $ ps_obls OP δ2 = dom $ ps_obls OP δ1) SAME.
+    add_case (dom $ ps_obls δ2 = dom $ ps_obls δ1) SAME.
     { intros EQ. red. by rewrite EQ. }
     
     red in LSTEP. destruct LSTEP as [T|[T|[T|[T|[T|T]]]]].
@@ -367,56 +270,9 @@ Section ObligationsRepr.
     - destruct T as (?&?&?&T). inversion T; subst.
       apply SAME. by destruct δ1.
   Qed.     
-    
-  (*   - destruct T as (?&T). inversion T; subst. *)
-  (*     red in OBLS_CORR.  *)
-  (*     destruct b1; [| set_solver]. destruct OBLS_CORR as (? & DOM1 & SUB). *)
-  (*     exists false. split; [| done]. *)
-  (*     red. split; auto. *)
-  (*     subst ps' new_obls0. destruct δ1; simpl in *. *)
-  (*     rewrite !dom_insert_L dom_delete_L. *)
-  (*     rewrite DOM1. *)
-  (*     rewrite difference_union_distr_l_L difference_diag_L union_empty_r_L. *)
-  (*     clear -H3 SUB. *)
-  (*     pose proof (ns_ndot_disj θ 0). *)
-  (*     pose proof (ns_ndot_disj θ 1). *)
-  (*     assert (fork_left θ ≠ fork_right θ). *)
-  (*     { apply ns_ndot_diff_disj. done. } *)
-  (*     rewrite difference_disjoint_L; [| set_solver]. *)
-  (*     rewrite union_assoc_L. rewrite (union_comm_L {[ _ ]} _).   
-      rewrite union_comm_L. rewrite difference_union_L. *)
-  (*     set_solver.  *)
-  (* Qed. *)
-
-  (* Lemma ghost_step_th_obls_pres' c τ δ1 δ2 *)
-  (*   (GSTEP: ghost_step OP δ1 τ δ2) *)
-  (*   (TH_OWN: threads_own_obls c δ1) *)
-  (*   (DOMτ: is_Some (from_locale c.1 τ)): *)
-  (*   threads_own_obls' c δ2 (dom (ps_phases _ δ2) ∖ dom (ps_phases _ δ1)).  *)
-  (* Proof. *)
-  (* Admitted.  *)
- 
-  (* Lemma progress_step_th_obls_pres' c τ δ1 δ2 *)
-  (*   (STEP: progress_step OP δ1 τ δ2) *)
-  (*   (TH_OWN: threads_own_obls c δ1) *)
-  (*   (DOMτ: is_Some (from_locale c.1 τ)): *)
-  (*   threads_own_obls' c δ2 (dom (ps_phases _ δ2) ∖ dom (ps_phases _ δ1)). *)
-  (* Proof. *)
-  (* Admitted. *)
-
-  (* Lemma locale_step_th_obls_pres c1 c2 τ δ *)
-  (*   (STEP: locale_step c1 (Some τ) c2) *)
-  (*   (TH_OWN: threads_own_obls c1 δ): *)
-  (*   threads_own_obls c2 δ. *)
-  (* Proof. *)
-  (*   destruct c1, c2.  *)
-  (*   red. intros. *)
-  (*   assert (forall δ, dom (ps_obls OP δ) = dom (ps_phases OP δ)) as DOM by admit. *)    
-  (*   eapply from_locale_step; eauto. *)
-  (* Qed.  *)
-       
+           
   Lemma progress_step_obls_pres δ1 τ δ2 R
-    (STEP: progress_step OP δ1 τ δ2)
+    (STEP: progress_step δ1 τ δ2)
     (TH_OWN: obls_eq δ1 R)
     (* (DOMτ: is_Some (from_locale c.1 τ)) *)
     :
@@ -435,33 +291,19 @@ Section ObligationsRepr.
     lia. 
   Qed.
 
-  Lemma obls_eq_init δ: obls_eq δ (dom $ ps_obls OP δ).
+  Lemma obls_eq_init δ: obls_eq δ (dom $ ps_obls δ).
   Proof. done. Qed. 
     
-  Lemma locale_nofork_step_obls_pres c1 c2 τ θ δ1 δ2
-    (STEP: locale_step c1 (Some τ) c2)
-    (TH_OWN: threads_own_obls c1 δ1)
-    (TRANS: progress_step OP δ1 θ δ2)
-    (NOFORK: locales_of_cfg c2 = locales_of_cfg c1)
-    :
-    threads_own_obls c2 δ2.
-  Proof.
-    destruct c1 as [tp1 σ1], c2 as [tp2 σ2].
-    red. rewrite NOFORK.
-    eapply progress_step_obls_pres in TRANS; [| apply obls_eq_init].
-    rewrite TRANS. done. 
-  Qed.
+  Definition dom_phases_obls δ := dom $ ps_phases δ = dom $ ps_obls δ. 
+  Definition phases_eq δ1 R := ps_phases δ1 = R.
 
-  Definition dom_phases_obls δ := dom $ ps_phases OP δ = dom $ ps_obls OP δ. 
-
-  Lemma loc_step_dpo_pres δ1 δ2 θ
-    (LSTEP: loc_step OP δ1 θ δ2)
-    (OBLS_CORR: dom_phases_obls δ1)
-    (* (DOMτ: is_Some (from_locale c.1 τ)): *)
+  Lemma loc_step_phases_pres δ1 δ2 θ R
+    (LSTEP: loc_step δ1 θ δ2)
+    (PHASES_CORR: phases_eq δ1 R)
     :
-    dom_phases_obls δ2.
+    phases_eq δ2 R.
   Proof using.
-    clear -LSTEP OBLS_CORR.
+    clear -LSTEP PHASES_CORR.
     red in LSTEP. destruct LSTEP as [T|[T|[T|[T|[T|T]]]]].
     - destruct T as (?&?&T). inversion T; subst.
       by destruct δ1. 
@@ -469,11 +311,11 @@ Section ObligationsRepr.
       by destruct δ1. 
     - destruct T as (?&T). inversion T; subst.
       destruct δ1. simpl in *.
-      subst new_obls0. red. rewrite dom_insert_L. simpl. set_solver. 
+      subst new_obls0. red. subst new_ps. simpl. set_solver. 
     - destruct T as (?&T). inversion T; subst.
       destruct δ1. simpl in *.  
       subst new_obls0. simpl.
-      red. rewrite dom_insert_L. set_solver. 
+      red. set_solver. 
     - destruct T as (?&?&?&?&T). inversion T; subst.
       by destruct δ1. 
     - destruct T as (?&?&?&T). inversion T; subst.
@@ -481,745 +323,74 @@ Section ObligationsRepr.
   Qed. 
 
   (* TODO: refactor *)
-  Lemma progress_step_dpo_pres δ1 τ δ2
-    (STEP: progress_step OP δ1 τ δ2)
-    (DPO: dom_phases_obls δ1)
+  Lemma loc_step_nsteps_phases_pres δ1 δ2 θ R n
+    (LSTEPS: relations.nsteps (fun p1 p2 => loc_step p1 θ p2) n δ1 δ2)
+    (PHASES_CORR: phases_eq δ1 R)
+    :
+    phases_eq δ2 R.
+  Proof.
+    generalize dependent δ2. induction n.
+    { simpl. intros ? ->%nsteps_0. done. }
+    intros ? (δ'&STEP1&STEP2)%rel_compose_nsteps_next.
+    apply IHn in STEP1. eapply loc_step_phases_pres; eauto.
+  Qed. 
+
+  (* TODO: refactor *)
+  Lemma progress_step_phases_pres δ1 τ δ2 R
+    (STEP: progress_step δ1 τ δ2)
+    (DPO: phases_eq δ1 R)
     (* (DOMτ: is_Some (from_locale c.1 τ)) *)
     :
-    dom_phases_obls δ2.
+    phases_eq δ2 R.
   Proof.
     red in STEP. destruct STEP as (n&?&STEP).
     eapply rel_compose_mono in STEP.
     2: reflexivity.
     1: apply rel_compose_nsteps_next in STEP.
     2: { do 2 red. intros. by left. }
-    (* clear -(* DOMτ *) OM STEP TH_OWN. *)
-    generalize dependent δ2. induction n.
-    { simpl. intros ? ?%nsteps_once_inv. by eapply loc_step_dpo_pres. }
-    intros ? (δ'&STEP1&STEP2)%rel_compose_nsteps_next.
-    apply IHn in STEP1. eapply loc_step_dpo_pres; eauto.
-    lia. 
+    eapply loc_step_nsteps_phases_pres; eauto.
   Qed.
 
-  (* Definition valid_bij_step *)
-  (*   (σ1: cfg Λ) (oζ: olocale Λ) (σ2: cfg Λ) *)
-  (*   (δ1: mstate OM) (ℓ: mlabel OM) (δ2: mstate OM) *)
-  (*   m1 m2 *)
-  (*   := *)
-  (*   exists ζ,  *)
-  (*     threads_own_obls σ1 δ1 m1 /\ *)
-  (*     threads_own_obls σ2 δ2 m2 /\  *)
-  (*     oζ = Some ζ /\ (ζ, ℓ) ∈ m1 /\ *)
-  (*     match decide (locales_of_cfg σ2 ∖ locales_of_cfg σ1 = ∅) with *)
-  (*     | left _ => m2 = m1 *)
-  (*     | right NEQ => *)
-  (*         let ζ' := proj1_sig $ finitary.set_choose_L' _ NEQ in *)
-  (*         m2 = (m1 ∖ {[ (ζ, ℓ) ]}) ∪ {[ (ζ, fork_left ℓ); (ζ', fork_right ℓ) ]} *)
-  (*     end. *)
+  Lemma phases_eq_init δ: phases_eq δ (ps_phases δ).
+  Proof. done. Qed. 
 
+  (* TODO: refactor *)
+  Lemma progress_step_dpo_pres δ1 τ δ2
+    (STEP: progress_step δ1 τ δ2)
+    (DPO: dom_phases_obls δ1)
+    :
+    dom_phases_obls δ2.
+  Proof.
+    red. erewrite progress_step_obls_pres; [| eauto| apply obls_eq_init].
+    erewrite progress_step_phases_pres; [| eauto| apply phases_eq_init]. 
+    apply DPO. 
+  Qed.
 
-  (* Lemma valid_bij_nofork_restore *)
-  (*   (σ1: cfg Λ) (ζ: locale Λ) (σ2: cfg Λ) *)
-  (*   (δ1: mstate OM) (ℓ: mlabel OM) (δ2: mstate OM) *)
-  (*   m1 *)
-  (*   (TH_OWN: threads_own_obls σ1 δ1 m1) *)
-  (*   (OBLS_EQ: dom $ ps_obls OP δ1 = dom $ ps_obls OP δ2) *)
-  (*   (STEP_LOCS: locales_of_cfg σ1 = locales_of_cfg σ2) *)
-  (*   (IN: (ζ, ℓ) ∈ m1) *)
-  (*   : *)
-  (*   exists m2, valid_bij_step σ1 (Some ζ) σ2 δ1 ℓ δ2 m1 m2. *)
-  (* Proof.  *)
-  (*   rewrite /valid_bij_step. *)
-  (*   exists m1, ζ. rewrite STEP_LOCS difference_diag_L. *)
-  (*   (* Set Printing All. *) *)
-  (*   rewrite decide_True_pi. *)
-  (*   split; auto. split; [| auto]. *)
-  (*   red. rewrite -OBLS_EQ -STEP_LOCS. done. *)
-  (* Qed.  *)
-      
-  Definition obls_valid_evolution_step
-    (σ1: cfg Λ) (oζ: olocale Λ) (σ2: cfg Λ)
-    (δ1: mstate OM) (ℓ: mlabel OM) (δ2: mstate OM) :=
-    (* exists m1 m2, *)
-      (* valid_bij_step σ1 oζ σ2 δ1 ℓ δ2 m1 m2 /\ *)
-      mtrans δ1 ℓ δ2 /\
-      oζ = Some ℓ                
-  .
-
-  Definition obls_si `{ObligationsGS Σ}
-    (σ: cfg Λ) (δ: mstate OM): iProp Σ :=
-    (* ∃ m,  *)
-      obls_msi δ ∗
-      ⌜ threads_own_obls σ δ (* m *)⌝ ∗
-      ⌜ dom_phases_obls δ ⌝
-      (* ∗ gset_bij_own_auth obls_bij (DfracOwn 1) m *)
-  . 
-
-  (* Definition thread_phase `{ObligationsGS Σ} (τ: locale Λ) (π: Phase): iProp Σ := *)
-  (*   gset_bij_own_elem obls_bij τ π.  *)
-
-  Definition obls_init_resource `{ObligationsGS Σ}
-    (δ: mstate OM) (_: unit): iProp Σ :=
-    own obls_cps (◯ (cps_repr $ ps_cps _ δ)) ∗
-    own obls_sigs (◯ (sig_map_repr $ ps_sigs _ δ)) ∗
-    own obls_obls (◯ (obls_map_repr $ ps_obls _ δ)) ∗
-    own obls_eps (◯ (eps_repr $ ps_eps _ δ)) ∗
-    own obls_phs (◯ (phases_repr $ ps_phases _ δ)) ∗
-    own obls_exc_lb (◯MN (ps_exc_bound _ δ))
-  .
-
-  (* Definition obls_si_init_resource `{ObligationsGS Σ}: iProp Σ := *)
-  (*   ∃ (τ: locale Λ), thread_phase τ nroot. *)
-
-  Definition obls_is_init_st (σ: cfg Λ) (δ: mstate OM) :=
-    (* exists τ0 e0, σ.1 = [e0] /\ from_locale σ.1 τ0 = Some e0 /\ *)
-    (*         dom (ps_obls OP δ) = {[ τ0 ]}.  *)
-    exists τ0,
-      let R := {[ τ0 ]} in
-      locales_of_cfg σ = R /\ dom $ ps_obls OP δ = R /\ dom $ ps_phases OP δ = R. 
-
-  Let obls_Σ: gFunctors := #[
-      GFunctor (authUR (gmultisetUR cpO));
-      GFunctor (authUR (gmapUR SignalId sstR));
-      GFunctor (authUR (gmapUR Locale (exclR (gsetR natO))));
-      GFunctor (authUR (gsetUR epO));
-      GFunctor (authUR (gmapUR Locale (exclR phO)));
-      GFunctor (mono_natUR);
-      GFunctor (gset_bijR (locale Λ) Phase)
-   ].
-
-  Definition cp `{ObligationsGS Σ} (ph: Phase) (deg: Degree): iProp Σ :=
-    own obls_cps (◯ (cps_repr ({[+ ((ph, deg)) +]}))). 
-
-  Definition cp_mul `{ObligationsGS Σ} ph deg n: iProp Σ :=
-    (* fold_right bi_sep (⌜ True ⌝)%I (repeat (cp ph deg) n).  *)
-    own obls_cps (◯ (n *: {[+ (ph, deg) +]})). 
-
-  Definition cps `{ObligationsGS Σ} (m: gmultiset (@CallPermission Degree)) : iProp Σ :=
-      own obls_cps (◯ (cps_repr m)). 
-
-  Definition sgn `{ObligationsGS Σ} (sid: SignalId) (l: Level) (ob: option bool): iProp Σ :=
-    own obls_sigs (◯ ({[ sid := (to_agree l, mbind (Some ∘ Excl) ob ) ]})).
-
-  Definition obls `{ObligationsGS Σ} τ (R: gset SignalId) :=
-    own obls_obls (◯ ({[ τ := Excl R]}: gmapUR Locale (exclR (gsetR natO)))).
-
-  Definition sgns_level_gt `{ObligationsGS Σ} (R: gset SignalId) lm: iProp Σ :=
-    [∗ set] s ∈ R, (∃ l, sgn s l None ∗ ⌜ opar_lvl_lt lm l ⌝). 
+  (* TODO: move *)
+  Global Instance phase_le_PreOrder: PreOrder phase_le.
+  Proof.
+    rewrite /phase_le. 
+    split.
+    - set_solver.
+    - red. set_solver.
+  Qed.         
   
-  Definition ep `{ObligationsGS Σ} (sid: SignalId) π d: iProp Σ :=
-    own obls_eps (◯ {[ (sid, π, d) ]}). 
-
-  Definition exc_lb `{ObligationsGS Σ} (n: nat) :=
-    own obls_exc_lb (mono_nat_lb n).
-
-  Definition th_phase_ge `{ObligationsGS Σ} ζ π: iProp Σ :=
-    ∃ π__max, own obls_phs (◯ (phases_repr {[ ζ := π__max]})) ∗ ⌜ phase_le π π__max⌝.
-
-  Program Definition ObligationsEM: ExecutionModel Λ OM :=
-    {| 
-      em_preGS := ObligationsPreGS;
-      em_GS := ObligationsGS;
-      em_Σ := obls_Σ;
-      em_valid_evolution_step := obls_valid_evolution_step;
-      em_thread_post Σ `{ObligationsGS Σ} := 
-        fun τ => (obls τ ∅)%I;
-      em_msi Σ `{ObligationsGS Σ} := obls_si;
-      em_init_param := unit; (* ? *)
-      em_init_resource Σ `{ObligationsGS Σ} := obls_init_resource;
-      em_is_init_st := obls_is_init_st;
-    |}.
-  Next Obligation.
-    solve_inG.
+  (* TODO: refactor *)
+  Definition phase_lt := strict phase_le.
+  
+  Lemma phase_lt_fork π (d: nat):
+    phase_lt π (π .@ d).
+  Proof.
+    red. split.
+    { apply nclose_subseteq. }
+    red. rewrite /phase_le.
+    (* TODO: make a lemma? *)
+    intros SUB. pose proof (nclose_subseteq π (d + 1)).
+    pose proof (coPpick_elem_of (↑π.@(d + 1)) (nclose_infinite _)) as IN.
+    edestruct @ndot_ne_disjoint; cycle 1. 
+    { apply IN. }
+    { apply SUB. apply H0. done. }
+    lia.
   Qed. 
-  Next Obligation.
-    simpl. intros ? PRE δ σ ? INIT. iStartProof.
-    iMod (own_alloc (● (cps_repr $ ps_cps _  δ) ⋅ ◯ _)) as (?) "[CPa CPf]".
-    { by apply auth_both_valid_2. }
-    iMod (own_alloc (● (sig_map_repr (ps_sigs _ δ)) ⋅ ◯ _)) as (?) "[SIGSa SIGSf]".
-    { apply auth_both_valid_2; [| reflexivity].
-      rewrite /sig_map_repr.
-      intros s. destruct lookup eqn:L; [| done].
-      apply lookup_fmap_Some in L. 
-      destruct L as ([l b]&<-&?).
-      done. }
-    iMod (own_alloc (● (obls_map_repr $ ps_obls _ δ) ⋅ ◯ _)) as (?) "[OBLSa OBLSf]". 
-    { apply auth_both_valid_discrete. split; [reflexivity| ].
-      intros τ. rewrite lookup_fmap. 
-      by destruct lookup. }
-    iMod (own_alloc (● (eps_repr $ ps_eps _ δ) ⋅ ◯ _)) as (?) "[EPSa EPSf]". 
-    { by apply auth_both_valid_2. }
-    iMod (own_alloc (● (phases_repr $ ps_phases _ δ) ⋅ ◯ _)) as (?) "[PHa PHf]". 
-    { apply auth_both_valid_2; [| reflexivity].
-      rewrite /phases_repr. intros τ. destruct lookup eqn:L; [| done].
-      rewrite lookup_fmap_Some in L. destruct L as (? & <- & L). done. }
-    iMod (own_alloc (●MN (ps_exc_bound _ δ) ⋅ mono_nat_lb _)) as (?) "[LBa LBf]".
-    { apply mono_nat_both_valid. reflexivity. }
-    iModIntro. iExists {| obls_pre := PRE; |}.
-    iFrame.
-    iPureIntro. 
-    red in INIT. destruct INIT as (?&?&?&?). set_solver.  
-  Qed.
-
-  (* Instance foo: SingletonMS (Phase * Degree) (gmultiset CallPermission).  *)
-  (* Existing Instance namespace_eq_dec.  *)
-  (* Existing Instance namespace_countable.  *)
-
-  (* Instance foo: SingletonMS (Phase * Degree) (gmultiset (@CallPermission Degree)). *)
-  (* apply gmultiset_singleton. *)
-  (* Defined.  *)
-    
-  Section ResourcesFacts.
-    Context `{ObligationsGS Σ}. 
-    
-    (* Global Instance th_phase_ge_Pers ζ π: Persistent (th_phase_ge ζ π). *)
-    
-    (* ⌜ ps_phases OP δ !! τ = Some π__max /\ phase_le ph π__max /\ *)
-    Lemma cp_msi_dom δ ph deg:
-      ⊢ obls_msi δ -∗ cp ph deg -∗
-        ⌜ (ph, deg) ∈ ps_cps OP δ ⌝.
-    Proof.
-      rewrite /obls_msi. iIntros "(CPS&_) CP". 
-      iCombine "CPS CP" as "CPS". 
-      iDestruct (own_valid with "[$]") as %V. iPureIntro.
-      apply auth_both_valid_discrete, proj1 in V.
-      apply gmultiset_singleton_subseteq_l.
-      by apply gmultiset_included.
-    Qed.
-
-    Lemma obls_msi_exact δ ζ R:
-      ⊢ obls_msi δ -∗ obls ζ R -∗
-        ⌜ ps_obls OP δ !! ζ = Some R ⌝.
-    Proof. 
-      rewrite /obls_msi. iIntros "(_&_&OBLS&_) OB". 
-      iCombine "OBLS OB" as "OBLS". 
-      iDestruct (own_valid with "[$]") as %V. iPureIntro.
-      apply auth_both_valid_discrete in V as [SUB V].
-      eapply singleton_included_exclusive_l in SUB; try done.
-      2: { apply _. }
-      apply leibniz_equiv_iff in SUB.
-      rewrite lookup_fmap_Some in SUB. destruct SUB as (?&?&?).
-      set_solver.
-    Qed. 
-
-    (* TODO: unify sigs_msi_.. proofs *)
-    Lemma sigs_msi_in δ sid l ov:
-      ⊢ obls_msi δ -∗ sgn sid l ov -∗
-        ⌜ exists v, ps_sigs OP δ !! sid = Some (l, v) ⌝.
-    Proof. 
-      rewrite /obls_msi. iIntros "(_&SIGS&_) SIG". 
-      iCombine "SIGS SIG" as "SIGS". 
-      iDestruct (own_valid with "[$]") as %V. iPureIntro.
-      apply auth_both_valid_discrete in V as [SUB V].
-      apply @singleton_included_l in SUB. destruct SUB as ([l' y]&SIG'&LE').
-
-      simpl in LE'. rewrite -SIG' in LE'.
-      rewrite /sig_map_repr in LE'.
-      rewrite lookup_fmap in LE'.
-      destruct (ps_sigs OP δ !! sid) as [[??]|] eqn:LL.
-      all: rewrite LL in LE'; simpl in LE'.
-      2: { apply option_included_total in LE' as [?|?]; set_solver. }
-      rewrite Some_included_total in LE'.
-      apply pair_included in LE' as [LE1 LE2].      
-      apply to_agree_included in LE1.
-      set_solver. 
-    Qed. 
-
-    Lemma sigs_msi_exact δ sid l v:
-      ⊢ obls_msi δ -∗ sgn sid l (Some v) -∗
-        ⌜ ps_sigs OP δ !! sid = Some (l, v) ⌝.
-    Proof. 
-      rewrite /obls_msi. iIntros "(_&SIGS&_) SIG". 
-      iCombine "SIGS SIG" as "SIGS". 
-      iDestruct (own_valid with "[$]") as %V. iPureIntro.
-      apply auth_both_valid_discrete in V as [SUB V].
-      apply @singleton_included_l in SUB. destruct SUB as ([l' y]&SIG'&LE').
-
-      simpl in LE'. rewrite -SIG' in LE'.
-      rewrite /sig_map_repr in LE'.
-      rewrite lookup_fmap in LE'.
-      destruct (ps_sigs OP δ !! sid) as [[??]|] eqn:LL.
-      all: rewrite LL in LE'; simpl in LE'.
-      2: { apply option_included_total in LE' as [?|?]; set_solver. }
-      rewrite Some_included_total in LE'.
-      apply pair_included in LE' as [LE1 LE2].      
-      apply to_agree_included in LE1.
-      apply Excl_included in LE2.
-      set_solver. 
-    Qed.
-
-    Instance sgn_ex_pers sid l: Persistent (sgn sid l None).
-    Proof. apply _. Qed.  
-
-    Lemma sgn_get_ex sid l ov:
-      ⊢ sgn sid l ov -∗ sgn sid l ov ∗ sgn sid l None. 
-    Proof.
-      iIntros "SIG". rewrite -own_op. iApply own_proper; [| done]. 
-      rewrite -auth_frag_op. rewrite gmap_op. simpl.
-      rewrite -!insert_empty. simpl.
-      erewrite <- insert_merge_r.
-      2: { rewrite insert_empty. rewrite lookup_singleton. done. }
-      rewrite fin_maps.RightId_instance_0.
-      rewrite insert_insert.
-      rewrite -pair_op. rewrite op_None_right_id.
-      rewrite agree_idemp. done.
-    Qed.
-
-    (* Global Instance sgns_level_gt_pers (R: gset SignalId) lm: *)
-    (*   Persistent (sgns_level_gt R lm). *)
-    (* Proof. apply _. Qed.  *)
-
-    (* Global Instance ep_pers sid π d: Persistent (ep sid π d). *)
-    (* Proof. apply _. Qed.  *)
-
-    Lemma th_phase_msi_ge_strong δ ζ π:
-      ⊢ obls_msi δ -∗ th_phase_ge ζ π -∗        
-        obls_msi δ ∗ ∃ π__max, own obls_phs (◯ phases_repr {[ζ := π__max]}) ∗ ⌜ ps_phases OP δ !! ζ = Some π__max /\ phase_le π π__max ⌝. 
-    Proof.
-      rewrite /obls_msi. iIntros "(?&?&?&?&PHASES&?) PH".
-      iRevert "PHASES PH". iFrame. iIntros "PHASES PH".  
-      rewrite /th_phase_ge. iDestruct "PH" as "(%π__max & PH & %LE)". 
-      iDestruct (own_valid with "[PHASES PH]") as "#V".
-      { iApply own_op. iApply bi.sep_comm. iFrame. }
-      iDestruct "V" as %V. 
-      iFrame. iExists _. iFrame. iPureIntro. 
-      split; eauto. 
-      apply auth_both_valid_discrete in V as [SUB V].
-      rewrite /phases_repr in SUB. rewrite map_fmap_singleton in SUB. 
-      apply @singleton_included_l in SUB. destruct SUB as (π'&PH'&LE').
-      destruct π' as [π'| ].
-      2: { specialize (V ζ). rewrite PH' in V. done. }
-      apply Excl_included in LE'.
-      rewrite -LE' in PH'.
-
-      apply leibniz_equiv_iff in PH'.
-      rewrite lookup_fmap_Some in PH'. by destruct PH' as (?&[=->]&?).
-    Qed.
-
-    Lemma th_phase_msi_ge δ ζ π:
-      ⊢ obls_msi δ -∗ th_phase_ge ζ π -∗        
-        ⌜ exists π__max, ps_phases OP δ !! ζ = Some π__max /\ phase_le π π__max ⌝. 
-    Proof.
-      iIntros "? ?". 
-      iDestruct (th_phase_msi_ge_strong with "[$] [$]") as "[? L]".
-      iDestruct "L" as (?) "[? %F]".
-      iPureIntro. eauto. 
-    Qed.
-
-    Lemma exc_lb_msi_bound δ n:
-      ⊢ obls_msi δ -∗ exc_lb n -∗ ⌜ n <= ps_exc_bound OP δ ⌝.
-    Proof.
-      rewrite /obls_msi. iIntros "(_&_&_&_&_&B) LB".
-      iCombine "B LB" as "LB".
-      iDestruct (own_valid with "LB") as %V. iPureIntro.
-      by apply mono_nat_both_valid in V.
-    Qed.
-
-    Lemma obls_sgn_lt_locale_obls δ ζ R lm:
-      ⊢ obls_msi δ -∗ obls ζ R -∗ sgns_level_gt R lm -∗
-        ⌜ lt_locale_obls OP lm ζ δ ⌝.
-    Proof.
-      (* rewrite /obls_msi. *)
-      iIntros "MSI OBLS SIGS_LT".
-      iDestruct (obls_msi_exact with "[$] [$]") as %Rζ. 
-      (* iIntros "(?&?&?&?&?&?) OBLS SIGS_LT". *)
-      rewrite /lt_locale_obls. rewrite Rζ. simpl.
-      rewrite -pure_forall_2. setoid_rewrite <- bi.pure_impl_2. 
-      iIntros (l [sid [-> IN]]%elem_of_map).
-      iDestruct (big_sepS_forall with "SIGS_LT") as "LT".
-      iSpecialize ("LT" $! _ IN). iDestruct "LT" as "(%l & SIG & %LT)".
-      iDestruct (sigs_msi_in with "[$] [$]") as %[? SIG]. rewrite SIG.
-      done.
-    Qed. 
-
-    (* Global Instance th_phase_ge_pers ζ π: Persistent (th_phase_ge ζ π). *)
-    (* Proof. apply _. Qed.  *)
-    
-    Lemma ep_msi_in δ sid π d:
-      ⊢ obls_msi δ -∗ ep sid π d -∗
-        ⌜ ((sid, π, d): (@ExpectPermission _)) ∈ (ps_eps OP δ) ⌝. 
-    Proof. 
-      rewrite /obls_msi. iIntros "(_&_&_&EPS&_) EP". 
-      iCombine "EPS EP" as "EPS". 
-      iDestruct (own_valid with "[$]") as %V. iPureIntro.
-      apply auth_both_valid_discrete in V as [SUB V].
-      by apply gset_included, singleton_subseteq_l in SUB.
-    Qed. 
-
-  End ResourcesFacts.
-
-  Section ResourcesUpdates.
-    Context `{ObligationsGS Σ}.
-
-    Let OU' (R: ProgressState OP -> Locale -> ProgressState OP -> Prop) ζ P: iProp Σ :=
-      ∀ δ, obls_msi δ ==∗ ∃ δ', obls_msi δ' ∗ ⌜ R δ ζ δ'⌝ ∗ P. 
-
-    Definition OU := OU' (loc_step OP). 
-
-    Lemma OU_wand ζ P Q:
-      (P -∗ Q) -∗ OU ζ P -∗ OU ζ Q.
-    Proof.
-      iIntros "PQ OU".
-      rewrite /OU /OU'. iIntros "**".
-      iSpecialize ("OU" with "[$]"). iMod "OU" as "(%&?&?&?)". iModIntro.
-      iExists _. iFrame. by iApply "PQ". 
-    Qed.
-        
-    Lemma OU_create_sig ζ R l:
-      ⊢ obls ζ R -∗ OU ζ (∃ sid, sgn sid l (Some false) ∗ obls ζ (R ∪ {[ sid ]})).
-    Proof.
-      rewrite /OU /OU'. iIntros "OB %δ MSI".
-      set (sid := list_max (elements $ dom $ sig_map_repr $ ps_sigs OP δ) + 1).
-      iDestruct (obls_msi_exact with "[$] [$]") as %Rζ. 
-      rewrite {1}/obls_msi. iDestruct "MSI" as "(?&SIGS&OBLS&?&?&?)".
-      destruct δ. simpl. iFrame. simpl in *.
-      iApply bupd_exist. iExists (Build_ProgressState _ _ _ _ _ _ _). 
-      iRevert "SIGS OBLS". iFrame. iIntros "SIGS OBLS". simpl.
-      rewrite !bi.sep_assoc. 
-
-      assert (sid ∉ dom ps_sigs0) as FRESH.
-      { subst sid. 
-        rewrite dom_fmap_L.
-        intros IN. apply elem_of_elements, elem_of_list_In in IN.
-        eapply List.Forall_forall in IN.
-        2: { apply list_max_le. reflexivity. }
-        simpl in IN. 
-        clear -IN. 
-        assert (forall n, n + 1 <= n -> False) as C by lia.
-        by apply C in IN. }
-
-      rewrite bi.sep_comm bi.sep_assoc.  
-      iSplitL.
-      2: { iPureIntro.
-           red. do 2 right. left. exists l. 
-           erewrite (f_equal (creates_signal _ _ _)).
-           { econstructor; eauto. simpl. eapply elem_of_dom; eauto. }
-           simpl. reflexivity. }
-
-      iMod (own_update with "[OB OBLS]") as "X".
-      2: iCombine "OBLS OB" as "?"; iFrame.
-      { apply auth_update.
-        apply singleton_local_update_any.
-        intros ? RR. apply lookup_fmap_Some in RR as (R_&?&Rζ_).
-        rewrite Rζ in Rζ_. inversion Rζ_. subst R_. subst.
-        apply exclusive_local_update with (x' := Excl (R ∪ {[sid]})). done. }
-      rewrite Rζ. simpl. iDestruct "X" as "[??]".
-      rewrite bi.sep_exist_r. iApply bupd_exist. iExists sid. 
-      rewrite -fmap_insert. iFrame.
-
-      rewrite -own_op. iApply own_update; [| by iFrame].
-      rewrite cmra_comm. apply auth_update_alloc. 
-      eapply local_update_proper.
-      1: reflexivity.
-      2: eapply alloc_local_update.
-      { rewrite /sig_map_repr. rewrite insert_empty fmap_insert. reflexivity. }
-      2: done.
-      apply not_elem_of_dom. by rewrite dom_fmap.
-    Qed. 
-
-    (* TODO: do we need to generalize to "optional v" instead? *)
-    Lemma OU_set_sig ζ R sid l v
-      (IN: sid ∈ R):
-      ⊢ obls ζ R -∗ sgn sid l (Some v) -∗
-        OU ζ (sgn sid l (Some true) ∗ obls ζ (R ∖ {[ sid ]})).
-    Proof.
-      rewrite /OU /OU'. iIntros "OB SIG %δ MSI".
-      iDestruct (sigs_msi_exact with "[$] [$]") as %Sζ.
-      iDestruct (obls_msi_exact with "[$] [$]") as %Rζ. 
-      rewrite {1}/obls_msi. iDestruct "MSI" as "(?&SIGS&OBLS&?&?&?)".
-      destruct δ. simpl in *.
-      iCombine "OBLS OB" as "OBLS". iCombine "SIGS SIG" as "SIGS".
-      iApply bupd_exist. iExists (Build_ProgressState _ _ _ _ _ _ _). 
-      iRevert "OBLS SIGS". iFrame. simpl. iIntros "OBLS SIGS".
-
-      rewrite bi.sep_comm -!bi.sep_assoc.  
-      iSplitR.
-      { iPureIntro.
-        red. do 3 right. left. exists sid. 
-        erewrite (f_equal (sets_signal _ _ _)).
-        { econstructor; eauto. simpl. eapply elem_of_dom; eauto. }
-        simpl. reflexivity. }
-      
-      iMod (own_update with "OBLS") as "OBLS".
-      { apply auth_update.
-        apply singleton_local_update_any.
-        intros ? RR. apply lookup_fmap_Some in RR as (R_&?&Rζ_).
-        rewrite Rζ in Rζ_. inversion Rζ_. subst R_. subst.
-        apply exclusive_local_update with (x' := Excl (R ∖ {[ sid ]})). 
-        done. }
-      iDestruct "OBLS" as "[??]". rewrite Rζ. simpl.
-      rewrite -fmap_insert. iFrame.
-
-      rewrite /sgn. rewrite bi.sep_comm. rewrite -!own_op.
-      iApply own_update; [| by iFrame].  
-      apply auth_update. simpl.
-      eapply local_update_proper.
-      1: reflexivity.
-      2: eapply singleton_local_update_any.
-      { rewrite /sig_map_repr. rewrite fmap_insert. reflexivity. }
-      intros ?. rewrite /sig_map_repr.
-      rewrite lookup_fmap_Some. intros [[??] [<- Sζ']].
-      rewrite Sζ in Sζ'. inversion Sζ'. subst.
-      apply prod_local_update'; [done| ].
-      apply option_local_update.  
-      by apply exclusive_local_update.
-    Qed.
-
-    Lemma exchange_cp_upd ζ π d d' b k
-      (LE: k <= b)
-      (DEG: opar_deg_lt d' d):
-      ⊢ cp π d -∗ th_phase_ge ζ π -∗ exc_lb b -∗ OU ζ (cp_mul π d' k ∗ th_phase_ge ζ π). 
-    Proof.
-      rewrite /OU /OU'. iIntros "CP PH #LB %δ MSI".
-      iDestruct (exc_lb_msi_bound with "[$] [$]") as %LB.
-      iDestruct (th_phase_msi_ge with "[$] [$]") as %(? & ? & ?).
-      iDestruct (cp_msi_dom with "[$] [$]") as %CP. 
-      rewrite {1}/obls_msi. iDestruct "MSI" as "(CPS&?&?&?&?&?)".
-      destruct δ. simpl in *.
-      iCombine "CPS CP" as "CPS".
-      iApply bupd_exist. iExists (Build_ProgressState _ _ _ _ _ _ _). 
-      iRevert "CPS". iFrame. simpl. iIntros "CPS".
-
-      rewrite bi.sep_comm -!bi.sep_assoc.  
-      iSplitR.
-      { iPureIntro.
-        red. right. left. exists π, d, d', k. 
-        erewrite (f_equal (exchanges_cp _ _ _)).
-        { econstructor; eauto. simpl. lia. }
-        simpl. reflexivity. }
-
-      rewrite /cps_repr. rewrite bi.sep_comm. rewrite /cp_mul /cp. rewrite -own_op.
-      iApply own_update; [| by iFrame].
-      apply auth_update.
-      etrans.
-      { eapply gmultiset_local_update_dealloc. reflexivity. }
-      rewrite gmultiset_difference_diag.
-      eapply local_update_proper.
-      1: reflexivity.
-      2: eapply gmultiset_local_update_alloc.
-      by rewrite gmultiset_disj_union_left_id. 
-    Qed.
-
-    (* TODO: ? use duplicable "signal exists" resource *)
-    Lemma create_ep_upd ζ π d d' sid l ov (DEG: opar_deg_lt d' d) 
-      :
-      ⊢ cp π d -∗ sgn sid l ov -∗ th_phase_ge ζ π -∗ 
-        OU ζ (ep sid π d' ∗ sgn sid l ov ∗ th_phase_ge ζ π).
-    Proof.
-      rewrite /OU /OU'. iIntros "CP SIG PH %δ MSI".
-      iDestruct (sigs_msi_in with "[$] [$]") as %[v Sζ].
-      iDestruct (th_phase_msi_ge with "[$] [$]") as %(? & ? & ?).
-      iDestruct (cp_msi_dom with "[$] [$]") as %CP. 
-      rewrite {1}/obls_msi. iDestruct "MSI" as "(CPS&SIGS&?&EPS&?&?)".
-      destruct δ. simpl in *.
-      iCombine "CPS CP" as "CPS".
-      iApply bupd_exist. iExists (Build_ProgressState _ _ _ _ _ _ _). 
-      iRevert "CPS EPS". iFrame. simpl. iIntros "CPS EPS".
-
-      rewrite bi.sep_comm -!bi.sep_assoc.
-      iSplitR.
-      { iPureIntro.
-        red. do 4 right. left. exists sid. do 3 eexists. 
-        erewrite (f_equal (creates_ep _ _ _)).
-        { econstructor; eauto.
-          simpl. by apply elem_of_dom. }
-        simpl. reflexivity. }
-
-      rewrite /ep. rewrite /cps_repr /eps_repr. 
-      rewrite bi.sep_comm -bi.sep_assoc.
-      
-      iMod (own_update with "EPS") as "EPS".
-      { apply auth_update_alloc.
-        eapply gset_local_update.
-        eapply union_subseteq_l. }
-      iSplitR "EPS".
-      2: { iDestruct "EPS" as "[A F]".
-           iSplitL "A".
-           { iApply "A". }           
-           iModIntro. iApply own_mono; [| by iFrame].
-           apply auth_frag_mono. apply gset_included. apply union_subseteq_r. }
-      
-      iApply own_update; [| by iFrame].
-      apply auth_update_dealloc.
-      eapply local_update_proper.
-      1: reflexivity.
-      2: { apply gmultiset_local_update_dealloc. reflexivity. }
-      rewrite gmultiset_difference_diag. set_solver.
-    Qed. 
-      
-    Lemma expect_sig_upd ζ sid π d l R
-      :
-      ⊢ ep sid π d -∗ sgn sid l (Some false) -∗ obls ζ R -∗
-        sgns_level_gt R l -∗ th_phase_ge ζ π -∗
-        OU ζ (cp π d ∗ sgn sid l (Some false) ∗ obls ζ R ∗ th_phase_ge ζ π).
-    Proof.
-      rewrite /OU /OU'. iIntros "#EP SIG OBLS #SIGS_LT PH %δ MSI".
-      iDestruct (sigs_msi_exact with "[$] [$]") as %Sζ.
-      iDestruct (th_phase_msi_ge with "[$] [$]") as %(? & ? & ?).
-      iDestruct (ep_msi_in with "[$] [$]") as %EP. 
-      iDestruct (obls_sgn_lt_locale_obls with "[$] [$] [$]") as %LT. 
-
-      rewrite {1}/obls_msi. iDestruct "MSI" as "(CPS&?&?&?&?&?)".
-      destruct δ. simpl in *.
-      iApply bupd_exist. iExists (Build_ProgressState _ _ _ _ _ _ _). 
-      iRevert "CPS". iFrame. simpl. iIntros "CPS".
-
-      rewrite /cp /cps_repr /eps_repr. 
-      rewrite bi.sep_comm -bi.sep_assoc.
-      iSplitR.
-      { iPureIntro.
-        red. do 5 right. do 3 eexists. 
-        erewrite (f_equal (expects_ep _ _ _)).
-        { econstructor; eauto. }
-        simpl. reflexivity. }
-
-      rewrite bi.sep_comm. rewrite -own_op.
-      iApply own_update; [| by iFrame].
-      apply auth_update_alloc.
-      eapply local_update_proper.
-      1: reflexivity.
-      2: eapply gmultiset_local_update_alloc.
-      f_equiv. rewrite gmultiset_disj_union_left_id. set_solver.
-    Qed. 
-
-    (* TODO: ? refactor these proofs about burn_cp *)
-    Lemma burn_cp_upd_impl δ ζ π deg
-      (PH_MAX: exists π__max, ps_phases OP δ !! ζ = Some π__max /\ phase_le π π__max)
-      :
-      ⊢ obls_msi δ -∗ cp π deg ==∗ ∃ δ', obls_msi δ' ∗ ⌜ burns_cp OP δ ζ δ' π deg⌝.
-    Proof.
-      iIntros "MSI CP".
-      iDestruct (cp_msi_dom with "[$] [$]") as "%IN". 
-      rewrite {1}/obls_msi. iDestruct "MSI" as "(CPS&?&?&?&?&?)".
-      destruct δ. simpl in *. iApply bupd_exist. iExists (Build_ProgressState _ _ _ _ _ _ _). 
-      simpl. iRevert "CPS". iFrame. iIntros "CPS". simpl.
-      rewrite /cp.
-      iCombine "CPS CP" as "CPS". iMod (own_update with "CPS").
-      { apply auth_update_dealloc.
-        eapply local_update_proper; [..| eapply gmultiset_local_update_dealloc].
-        1, 3: reflexivity.
-        f_equiv. by rewrite gmultiset_difference_diag. }
-      iModIntro. iFrame. iPureIntro.
-      destruct PH_MAX as (?&?&?). 
-      erewrite (f_equal (burns_cp _ _ _)).
-      { econstructor; eauto. }
-      done. 
-    Qed.
-
-    Lemma burn_cp_upd_burn ζ π deg:
-      ⊢ cp π deg -∗ th_phase_ge ζ π -∗ 
-        OU' (fun δ1 ζ' δ2 => burns_cp OP δ1 ζ' δ2 π deg) ζ (th_phase_ge ζ π). 
-    Proof.
-      rewrite /OU'. iIntros "CP PH % MSI".
-      iDestruct (th_phase_msi_ge with "[$] [$]") as %(? & ? & ?). 
-      iMod (burn_cp_upd_impl with "[$] [$]") as "R"; eauto.
-      iDestruct "R" as "(%&?&?)". iModIntro. iExists _. iFrame.
-    Qed.
-
-    Lemma burn_cp_upd ζ π deg:
-      ⊢ cp π deg -∗ th_phase_ge ζ π -∗ OU ζ (th_phase_ge ζ π). 
-    Proof.
-      iIntros "??".
-      iPoseProof (burn_cp_upd_burn with "[$] [$]") as "OU'".
-      rewrite /OU /OU'. iIntros "% MSI".
-      iMod ("OU'" with "[$]") as "(%&?&%&?)". iModIntro.
-      iExists _. iFrame. iPureIntro.
-      red. eauto.
-    Qed. 
-
-    Lemma cp_mul_take ph deg n:
-      cp_mul ph deg (S n) ⊣⊢ cp_mul ph deg n ∗ cp ph deg.
-    Proof. 
-      rewrite /cp_mul. rewrite -own_op -auth_frag_op. 
-      iApply own_proper. f_equiv.
-      rewrite gmultiset_op.
-      by rewrite gmultiset_scalar_mul_S_r. 
-    Qed.
-
-    (* TODO: refactor *)
-    Definition phase_lt π1 π2 := phase_le π1 π2 /\ π1 ≠ π2.
-
-    (* TODO: make an instance*)
-    Lemma phase_le_refl π: phase_le π π.
-    Proof. set_solver. Qed. 
-
-    (* TODO: ? refactor these proofs about fork step *)
-    Lemma fork_locale_upd_impl δ ζ ζ' π R0 R'
-      (FRESH: ζ' ∉ dom $ ps_phases OP δ)
-      (DOM_EQ: dom_phases_obls δ)
-      :
-      ⊢ obls_msi δ -∗ th_phase_ge ζ π -∗ obls ζ R0 ==∗ 
-        ∃ δ' π1 π2, obls_msi δ' ∗ th_phase_ge ζ π1 ∗ th_phase_ge ζ' π2 ∗
-                    obls ζ (R0 ∖ R') ∗ obls ζ' R' ∗
-                    ⌜ forks_locale OP δ ζ δ' ζ' R' ⌝.
-    Proof.
-      iIntros "MSI PH OB".
-      iDestruct (th_phase_msi_ge_strong with "[$] [$]") as "(MSI & %π0 & (PH & %PH & %PLE))".
-      iDestruct (obls_msi_exact with "[$] [$]") as %OBLS. 
-      rewrite {1}/obls_msi. iDestruct "MSI" as "(?&?&OBLS&?&PHASES&?)".
-      destruct δ. simpl in *. iApply bupd_exist. iExists (Build_ProgressState _ _ _ _ _ _ _). 
-      simpl. iRevert "OBLS PHASES". iFrame. iIntros "OBLS PHASES". simpl.
-      iCombine "OBLS OB" as "OBLS". iCombine "PHASES PH" as "PHASES".
-      iExists (fork_left π0), (fork_right π0).
-
-      rewrite !bi.sep_assoc. iSplitL.
-      2: { iPureIntro.
-           erewrite (f_equal (forks_locale _ _ _)).
-           { econstructor; eauto. }
-           simpl. reflexivity. }
-
-      rewrite !OBLS. simpl.  
-      rewrite -(bi.sep_assoc _ _ (obls _ _)). rewrite bi.sep_comm.
-      rewrite -!bi.sep_assoc.
-      do 2 rewrite bi.sep_assoc. 
-      rewrite -bupd_sep. 
-      iSplitL "OBLS". 
-      - rewrite -!own_op. iApply own_update; [| by iFrame].
-        rewrite -auth_frag_op. rewrite (cmra_comm (◯ _) _).
-        etrans.
-        2: { rewrite auth_frag_op.
-             rewrite (cmra_comm (◯ _) _). rewrite cmra_assoc cmra_comm.
-             apply cmra_update_op; [reflexivity| ].
-             apply auth_update_alloc.
-             rewrite /obls_map_repr. rewrite fmap_insert.
-             apply alloc_singleton_local_update; [| done].
-             apply not_elem_of_dom. rewrite dom_fmap dom_insert_L.
-             rewrite not_elem_of_union not_elem_of_singleton. split.
-             - intros ->. destruct FRESH. by apply elem_of_dom.
-             - by rewrite -DOM_EQ. }
-        rewrite (cmra_comm (◯ _) _).
-        apply auth_update.
-        rewrite fmap_insert. apply singleton_local_update_any.
-        intros. apply exclusive_local_update. done.
-      - rewrite /th_phase_ge.
-        rewrite !bi.sep_exist_l; iExists _.
-        rewrite !bi.sep_assoc. iSplitL.
-        2: { iPureIntro. apply phase_le_refl. }
-        rewrite bi.sep_comm.
-        rewrite !bi.sep_exist_l; iExists _.
-        rewrite !bi.sep_assoc. iSplitL.
-        2: { iPureIntro. apply phase_le_refl. }
-        rewrite -bi.sep_assoc bi.sep_comm.
-        rewrite -!own_op. iApply own_update; [| by iFrame].
-        etrans.
-        2: { rewrite cmra_comm. rewrite cmra_assoc.
-             apply cmra_update_op; [| reflexivity].
-             rewrite cmra_comm. apply auth_update_alloc.
-             rewrite /phases_repr !fmap_insert. 
-             rewrite fmap_empty insert_empty.
-             apply alloc_singleton_local_update; [| done].
-             apply not_elem_of_dom. rewrite dom_insert_L dom_fmap.
-             rewrite not_elem_of_union not_elem_of_singleton. split.
-             - intros ->. destruct FRESH. by apply elem_of_dom.
-             - done. }
-        apply auth_update.
-        rewrite /phases_repr !fmap_insert. 
-        rewrite fmap_empty insert_empty.
-        apply singleton_local_update_any.
-        intros. eapply exclusive_local_update. done.
-        Unshelve. apply excl_exclusive.
-    Qed.
-
-  End ResourcesUpdates.
-
-End ObligationsRepr.
+  
+End Model.
